matching-logic/src/SyntacticConstruct.v
@@ -368,6 +368,161 @@ Proof.
   exact H.
 Qed.
 
+Class Ternary (ternary : Pattern -> Pattern -> Pattern -> Pattern) := {
+    ternary_morphism :
+      forall {A : Type} (f : A -> Pattern -> Pattern) (f_morph : PatternMorphism f) (phi1 phi2 phi3 : Pattern) a,
+        f a (ternary phi1 phi2 phi3) =
+          ternary (f a phi1) (f a phi2) (f a phi3);
+    ternary_wfp :
+      forall (ψ1 ψ2 ψ3: Pattern),
+        well_formed_positive (ternary ψ1 ψ2 ψ3)
+        = well_formed_positive ψ1 &&
+          well_formed_positive ψ2 &&
+          well_formed_positive ψ3 ;
+    ternary_wfcex :
+      forall (n : nat) (ψ1 ψ2 ψ3 : Pattern),
+            well_formed_closed_ex_aux (ternary ψ1 ψ2 ψ3) n
+            = well_formed_closed_ex_aux ψ1 n &&
+              well_formed_closed_ex_aux ψ2 n &&
+              well_formed_closed_ex_aux ψ3 n  ;
+    ternary_wfcmu :
+      forall (n : nat) (ψ1 ψ2 ψ3 : Pattern),
+            well_formed_closed_mu_aux (ternary ψ1 ψ2 ψ3) n
+            = well_formed_closed_mu_aux ψ1 n &&
+              well_formed_closed_mu_aux ψ2 n &&
+              well_formed_closed_mu_aux ψ3 n;
+}.
+
+Lemma ternary_wfxy
+  (ternary : Pattern -> Pattern -> Pattern -> Pattern)
+  {_b : Ternary ternary}
+:
+forall (x y : nat) (ψ1 ψ2 ψ3 : Pattern),
+  well_formed_xy x y (ternary ψ1 ψ2 ψ3)
+  = well_formed_xy x y ψ1 && well_formed_xy x y ψ2 && well_formed_xy x y ψ3.
+Proof.
+  unfold well_formed_xy.
+  intros.
+  rewrite ternary_wfp.
+  rewrite ternary_wfcex.
+  rewrite ternary_wfcmu.
+  btauto.
+Qed.
+
+Lemma ternary_wfxy_compose
+  (ternary : Pattern -> Pattern -> Pattern -> Pattern)
+  {_b : Ternary ternary}
+:
+forall (x y : nat) (ψ1 ψ2 ψ3 : Pattern),
+  well_formed_xy x y ψ1 = true /\
+  well_formed_xy x y ψ2 = true /\
+  well_formed_xy x y ψ3 = true ->
+  well_formed_xy x y (ternary ψ1 ψ2 ψ3) = true
+.
+Proof.
+  intros x y ψ1 ψ2 ψ3 H.
+  rewrite ternary_wfxy.
+  destruct H as [H1 [H2 H3] ].
+  rewrite H1 H2 H3.
+  reflexivity.
+Qed.
+
+Lemma ternary_wfxy_decompose
+  (ternary : Pattern -> Pattern -> Pattern -> Pattern)
+  {_b : Ternary ternary}
+:
+forall (x y : nat) (ψ1 ψ2 ψ3 : Pattern),
+  well_formed_xy x y (ternary ψ1 ψ2 ψ3) = true ->
+  well_formed_xy x y ψ1 = true /\ well_formed_xy x y ψ2 = true /\ well_formed_xy x y ψ3 = true
+.
+Proof.
+  intros x y ψ1 ψ2 ψ3 H.
+  rewrite ternary_wfxy in H.
+  apply andb_true_iff in H as [H ?].
+  apply andb_true_iff in H as [? ?].
+  firstorder.
+Qed.
+
+Class Quaternary (quaternary : Pattern -> Pattern -> Pattern -> Pattern -> Pattern) := {
+    quaternary_morphism :
+      forall {A : Type} (f : A -> Pattern -> Pattern) (f_morph : PatternMorphism f) (phi1 phi2 phi3 phi4 : Pattern) a,
+        f a (quaternary phi1 phi2 phi3 phi4) =
+          quaternary (f a phi1) (f a phi2) (f a phi3) (f a phi4);
+    quaternary_wfp :
+      forall (ψ1 ψ2 ψ3 ψ4: Pattern),
+        well_formed_positive (quaternary ψ1 ψ2 ψ3 ψ4)
+        = well_formed_positive ψ1 &&
+          well_formed_positive ψ2 &&
+          well_formed_positive ψ3 &&
+          well_formed_positive ψ4 ;
+    quaternary_wfcex :
+      forall (n : nat) (ψ1 ψ2 ψ3 ψ4 : Pattern),
+            well_formed_closed_ex_aux (quaternary ψ1 ψ2 ψ3 ψ4) n
+            = well_formed_closed_ex_aux ψ1 n &&
+              well_formed_closed_ex_aux ψ2 n &&
+              well_formed_closed_ex_aux ψ3 n &&
+              well_formed_closed_ex_aux ψ4 n  ;
+    quaternary_wfcmu :
+      forall (n : nat) (ψ1 ψ2 ψ3 ψ4 : Pattern),
+            well_formed_closed_mu_aux (quaternary ψ1 ψ2 ψ3 ψ4) n
+            = well_formed_closed_mu_aux ψ1 n &&
+              well_formed_closed_mu_aux ψ2 n &&
+              well_formed_closed_mu_aux ψ3 n &&
+              well_formed_closed_mu_aux ψ4 n;
+}.
+
+Lemma quaternary_wfxy
+  (quaternary : Pattern -> Pattern -> Pattern -> Pattern -> Pattern)
+  {_b : Quaternary quaternary}
+:
+forall (x y : nat) (ψ1 ψ2 ψ3 ψ4 : Pattern),
+  well_formed_xy x y (quaternary ψ1 ψ2 ψ3 ψ4)
+  = well_formed_xy x y ψ1 && well_formed_xy x y ψ2 && well_formed_xy x y ψ3 && well_formed_xy x y ψ4.
+Proof.
+  unfold well_formed_xy.
+  intros.
+  rewrite quaternary_wfp.
+  rewrite quaternary_wfcex.
+  rewrite quaternary_wfcmu.
+  btauto.
+Qed.
+
+Lemma quaternary_wfxy_compose
+  (quaternary : Pattern -> Pattern -> Pattern -> Pattern -> Pattern)
+  {_b : Quaternary quaternary}
+:
+forall (x y : nat) (ψ1 ψ2 ψ3 ψ4 : Pattern),
+  well_formed_xy x y ψ1 = true /\
+  well_formed_xy x y ψ2 = true /\
+  well_formed_xy x y ψ3 = true /\
+  well_formed_xy x y ψ4 = true ->
+  well_formed_xy x y (quaternary ψ1 ψ2 ψ3 ψ4) = true
+.
+Proof.
+  intros x y ψ1 ψ2 ψ3 ψ4 H.
+  rewrite quaternary_wfxy.
+  destruct H as [H1 [H2 [H3 H4] ] ].
+  rewrite H1 H2 H3 H4.
+  reflexivity.
+Qed.
+
+Lemma quaternary_wfxy_decompose
+  (quaternary : Pattern -> Pattern -> Pattern -> Pattern -> Pattern)
+  {_b : Quaternary quaternary}
+:
+forall (x y : nat) (ψ1 ψ2 ψ3 ψ4 : Pattern),
+  well_formed_xy x y (quaternary ψ1 ψ2 ψ3 ψ4) = true ->
+  well_formed_xy x y ψ1 = true /\ well_formed_xy x y ψ2 = true /\ well_formed_xy x y ψ3 = true /\ well_formed_xy x y ψ4 = true
+.
+Proof.
+  intros x y ψ1 ψ2 ψ3 ψ4 H.
+  rewrite quaternary_wfxy in H.
+  do 2 apply andb_true_iff in H as [H ?].
+  apply andb_true_iff in H as [? ?].
+  firstorder.
+Qed.
+
+
 Class Unary (unary : Pattern -> Pattern) := {
     unary_morphism :
       forall {A : Type} (f : A -> Pattern -> Pattern) (f_morph : PatternMorphism f) (phi : Pattern) a,
